rename Interp => Elaborate

theories/Elaborate.v
@@ -25,7 +25,7 @@ Notation "κ ∷ σ" := (Env.cons κ σ) (at level 30).
 
 Reserved Notation "⟦ M ⟧ κs" (at level 50).
 
-Fixpoint interp_tm `(M : Expr.t Λ Ψ) (κs : Env.t Λ) : Prog.t Ψ :=
+Fixpoint elab_tm `(M : Expr.t Λ Ψ) (κs : Env.t Λ) : Prog.t Ψ :=
   match M with
   | Expr.var i => Prog.var i
   | Expr.fst M => ⟦M⟧ κs .1
@@ -45,20 +45,20 @@ Fixpoint interp_tm `(M : Expr.t Λ Ψ) (κs : Env.t Λ) : Prog.t Ψ :=
   | Expr.lam M => 𝛌{⟦M⟧ κs}
   | Expr.app M1 M2 => ⟦M1⟧ κs ⋅ ⟦M2⟧ κs
   end
-where "⟦ M ⟧ κs" := (interp_tm M%etm κs) : prog_scope.
+where "⟦ M ⟧ κs" := (elab_tm M%etm κs) : prog_scope.
 
-Arguments interp_tm [Λ Ψ] M%etm κs.
+Arguments elab_tm [Λ Ψ] M%etm κs.
 
-Program Fixpoint interp_ctx `(Γ : ECtx.t Λ Ψ) (κs : Env.t Λ) : Prectx Ψ :=
+Program Fixpoint elab_ctx `(Γ : ECtx.t Λ Ψ) (κs : Env.t Λ) : Prectx Ψ :=
   match Γ with
   | ⋄%ectx => ⋄%ictx
   | (Γ ∙ A)%ectx => (⟦ Γ ⟧ κs ∙ ⟦ A ⟧ κs)%ictx
   end
-where "⟦ Γ ⟧ κs" := (interp_ctx Γ%ectx κs) : ctx_scope.
+where "⟦ Γ ⟧ κs" := (elab_ctx Γ%ectx κs) : ctx_scope.
 
-Arguments interp_ctx [Λ Ψ] Γ%ectx κs.
+Arguments elab_ctx [Λ Ψ] Γ%ectx κs.
 
-Definition interp_jdg `(J : EJdg.t Λ) : Ω :=
+Definition elab_jdg `(J : EJdg.t Λ) : Ω :=
   ∀ κs,
     match J with
     | ⌊ _ ∣ Γ ≫ A ∋ M1 ≐ M2 ⌋ =>
@@ -69,20 +69,20 @@ Definition interp_jdg `(J : EJdg.t Λ) : Ω :=
       (⟦ M1 ⟧ κs) ≈ (⟦ M2 ⟧ κs)
     end.
 
-Arguments interp_jdg [Λ] J%ejdg.
-Notation "⟦ J ⟧" := (interp_jdg J%ejdg) (at level 50) : type_scope.
+Arguments elab_jdg [Λ] J%ejdg.
+Notation "⟦ J ⟧" := (elab_jdg J%ejdg) (at level 50) : type_scope.
 
 
-Definition interp_subst `(σ : @Sub.t (Expr.t Λ) Ψ0 Ψ1) (κs : Env.t Λ) : @Sub.t Prog.t Ψ0 Ψ1 :=
+Definition elab_subst `(σ : @Sub.t (Expr.t Λ) Ψ0 Ψ1) (κs : Env.t Λ) : @Sub.t Prog.t Ψ0 Ψ1 :=
   fun x =>
     (⟦ σ x ⟧ κs)%prog.
 
-Notation "⟦ σ ⟧ κs" := (interp_subst σ%esubst κs) : subst_scope.
+Notation "⟦ σ ⟧ κs" := (elab_subst σ%esubst κs) : subst_scope.
 
 Local Open Scope prog_scope.
 Local Open Scope program_scope.
 
-Theorem interp_tm_clk_naturality {Λ1 Λ2 Ψ} (M : Expr.t Λ1 Ψ) (ρ : Ren.t Λ1 Λ2) (κs : Env.t Λ2) :
+Theorem elab_tm_clk_naturality {Λ1 Λ2 Ψ} (M : Expr.t Λ1 Ψ) (ρ : Ren.t Λ1 Λ2) (κs : Env.t Λ2) :
   ⟦ M ⟧ κs ∘ ρ = ⟦ M.⦃ρ⦄ ⟧ κs.
 Proof.
   move: Λ2 ρ κs; elim M => *;
@@ -98,15 +98,15 @@ Proof.
   by dependent induction x.
 Qed.
 
-Theorem interp_ctx_clk_naturality {Λ1 Λ2 Ψ} (Γ : ECtx.t Λ1 Ψ) (ρ : Ren.t Λ1 Λ2) (κs : Env.t Λ2) :
+Theorem elab_ctx_clk_naturality {Λ1 Λ2 Ψ} (Γ : ECtx.t Λ1 Ψ) (ρ : Ren.t Λ1 Λ2) (κs : Env.t Λ2) :
   (⟦ Γ ⟧ κs ∘ ρ)%ictx = (⟦ Γ.⦃ρ⦄ ⟧ κs)%ictx.
 Proof.
   induction Γ; simpl; auto.
-  rewrite interp_tm_clk_naturality.
+  rewrite elab_tm_clk_naturality.
   T.rewrites.
 Qed.
 
-Theorem interp_tm_var_naturality {Λ Ψ0 Ψ1 Ψ2} (M : Expr.t Λ Ψ0) (σ : Sub.t Ψ1 Ψ2) ρ κs :
+Theorem elab_tm_var_naturality {Λ Ψ0 Ψ1 Ψ2} (M : Expr.t Λ Ψ0) (σ : Sub.t Ψ1 Ψ2) ρ κs :
   (⟦ M ⟧ κs) ⫽ (σ ∘ ρ) = (⟦ M.[ρ] ⟧ κs) ⫽ σ.
 Proof.
   move: Ψ1 Ψ2 σ ρ κs.
@@ -119,18 +119,18 @@ Proof.
 Qed.
 
 
-Theorem interp_tm_var_ren_naturality {Λ Ψ0 Ψ1} (M : Expr.t Λ Ψ0) (ρ : Ren.t Ψ0 Ψ1) κs :
+Theorem elab_tm_var_ren_naturality {Λ Ψ0 Ψ1} (M : Expr.t Λ Ψ0) (ρ : Ren.t Ψ0 Ψ1) κs :
   (⟦ M ⟧ κs).[ ρ ] = (⟦ M.[ρ] ⟧ κs).
 Proof.
   by rewrite
      -(Prog.subst_ret (⟦ M .[ ρ] ⟧ κs))
      -(Prog.subst_ret (⟦ M ⟧ κs .[ρ]))
      Prog.subst_ren_coh
-     interp_tm_var_naturality.
+     elab_tm_var_naturality.
 Qed.
 
 
-Lemma interp_subst_cong_coh {Λ Ψ0 Ψ1 Ψ2} (σ01 : @Sub.t (Expr.t Λ) Ψ0 Ψ1) (σ12 : @Sub.t Prog.t Ψ1 Ψ2) (κs : Env.t Λ) :
+Lemma elab_subst_cong_coh {Λ Ψ0 Ψ1 Ψ2} (σ01 : @Sub.t (Expr.t Λ) Ψ0 Ψ1) (σ12 : @Sub.t Prog.t Ψ1 Ψ2) (κs : Env.t Λ) :
   (Sub.cong σ12 ◎ ⟦ Sub.cong σ01 ⟧ κs)%subst =
   Sub.cong (σ12 ◎ ⟦ σ01 ⟧ κs)%subst.
 Proof.
@@ -138,10 +138,10 @@ Proof.
   dependent induction x.
   - eauto.
   - simplify_subst.
-    by rewrite -interp_tm_var_naturality.
+    by rewrite -elab_tm_var_naturality.
 Qed.
 
-Theorem interp_tm_subst_naturality {Λ Ψ0 Ψ1 Ψ2} (M : Expr.t Λ Ψ0) (σ12 : Sub.t Ψ1 Ψ2) (σ01 : Sub.t Ψ0 Ψ1) κs :
+Theorem elab_tm_subst_naturality {Λ Ψ0 Ψ1 Ψ2} (M : Expr.t Λ Ψ0) (σ12 : Sub.t Ψ1 Ψ2) (σ01 : Sub.t Ψ0 Ψ1) κs :
   (⟦ M ⟧ κs) ⫽ (σ12 ◎ ⟦ σ01 ⟧ κs) = (⟦ M ⫽ σ01 ⟧ κs) ⫽ σ12.
 Proof.
   symmetry.
@@ -149,13 +149,13 @@ Proof.
   induction M; eauto; simpl;
   T.rewrites_with
     ltac:(repeat f_equal; try (T.eqcd; intros);
-          try rewrite /interp_subst /Expr.wk_sub;
-          try rewrite interp_subst_cong_coh;
+          try rewrite /elab_subst /Expr.wk_sub;
+          try rewrite elab_subst_cong_coh;
           Program.simplify_subst;
-          try rewrite -interp_tm_clk_naturality).
+          try rewrite -elab_tm_clk_naturality).
 Qed.
 
-Theorem interp_tm_ren_naturality {Λ0 Λ1 Ψ0 Ψ1 Ψ2} (M : Expr.t Λ0 Ψ0) (ρΛ : Ren.t Λ0 Λ1) (ρΨ : Ren.t Ψ0 Ψ1) (σ : Sub.t Ψ1 Ψ2) κs :
+Theorem elab_tm_ren_naturality {Λ0 Λ1 Ψ0 Ψ1 Ψ2} (M : Expr.t Λ0 Ψ0) (ρΛ : Ren.t Λ0 Λ1) (ρΨ : Ren.t Ψ0 Ψ1) (σ : Sub.t Ψ1 Ψ2) κs :
   (⟦ M ⟧ κs ∘ ρΛ) ⫽ (σ ∘ ρΨ) = (⟦ M.⦃ρΛ⦄[ρΨ] ⟧ κs) ⫽ σ.
 Proof.
   symmetry.
@@ -165,9 +165,9 @@ Proof.
   T.rewrites_with
     ltac:(repeat f_equal; try (T.eqcd; intros);
           try rewrite /Expr.wk_sub;
-          try rewrite interp_subst_cong_coh;
+          try rewrite elab_subst_cong_coh;
           simplify_subst;
-          try rewrite -interp_tm_clk_naturality;
+          try rewrite -elab_tm_clk_naturality;
           try rewrite -Sub.cong_coh_ptwise).
 
   by dependent induction x0.
